src/Crypto/Digests.dfy
@@ -1,0 +1,15 @@
+include "../Util/StandardLibrary.dfy"
+
+module {:extern "Digests"} Digests {
+  import opened StandardLibrary
+
+  datatype {:extern "HMAC_ALGORITHM"} HMAC_ALGORITHM = HmacSHA256 | HmacSHA384 | HmacNOSHA
+  
+  // Hash length in octets, e.g. HashLength(SHA256) = 256 = 32 * 8
+  function {:axiom} HashLength(algorithm: HMAC_ALGORITHM): nat
+    ensures algorithm == HmacSHA256 ==> HashLength(algorithm) == 32
+    ensures algorithm == HmacSHA384 ==> HashLength(algorithm) == 48
+
+  function {:axiom} Hash(algorithm: HMAC_ALGORITHM, key: seq<byte>, message: seq<byte>): seq<byte>
+    ensures |Hash(algorithm, key, message)| == HashLength(algorithm)
+}
