src/Util/StandardLibrary.dfy
@@ -1,0 +1,18 @@
+module {:extern "STL"} StandardLibrary {
+  datatype {:extern} Option<T> = None | Some(get: T)
+
+  newtype byte = x | 0 <= x < 256
+  type uint8 = byte
+
+  newtype int32 = x | -0x8000_0000 <= x < 0x8000_0000
+
+  newtype uint32 = x | 0 <= x < 0x1_0000_0000
+
+  function Fill<T>(value: T, n: nat): seq<T>
+    ensures |Fill(value, n)| == n
+    ensures forall i :: 0 <= i < n ==> Fill(value, n)[i] == value
+  {
+    if n > 0 then [value] + Fill(value, n-1) else []
+  }
+
+}
